FailureData + imported two parsers

src/Parsers/exampleArithmetic.dfy
@@ -1,73 +1,8 @@
 include "parser.dfy"
 
-module {:options "-functionSyntax:4", "-quantifierSyntax:4"}  EngineParens {
-  import opened Parsers
-  import opened ParserBuilders
-  import opened ParserEngine
-
-  class EngineParens extends ParserEngine.Engine {
-    constructor(input: string) {
-      this.input := input;
-    }
-
-    const fixmapBase: map<string, ParserMapper<Expression>> := map[]
-
-    function {:opaque} atom(functions: set<string>): (mapper: ParserMapper<Expression>)
-      requires "plus__" in functions
-      ensures RecSpecOnce("atom", functions, mapper)
-    {
-      (rec: ParserSelector<Expression>, pos: nat) requires RecSpec("atom", functions, rec, pos) =>
-        C?("(").o_I(B(rec("plus__")).I_o(C(")")))
-        .O(N().M(n => Number(n))).apply(pos)
-    }
-
-    function {:opaque} times(functions: set<string>): (mapper: ParserMapper<Expression>)
-      requires "atom" in functions
-      ensures RecSpecOnce("times", functions, mapper)
-    {
-      (rec: ParserSelector<Expression>, pos: nat) requires RecSpec("times", functions, rec, pos) =>
-       Bind(rec("atom"), (expr: Expression, pos': nat) =>
-             RepAcc(Concat(Or(Const?("*"), Or(Const?("/"), Const?("%"))), rec("atom")), expr, Expression.InfixBuilder()))(pos)
-    }
-
-    function {:opaque} plus(functions: set<string>): (mapper: ParserMapper<Expression>)
-      requires "times" in functions
-      ensures RecSpecOnce("plus__", functions, mapper)
-    {
-      (rec: ParserSelector<Expression>, pos: nat) requires RecSpec("plus__", functions, rec, pos) =>
-       Bind(rec("times"), (expr: Expression, pos': nat) =>
-             RepAcc(Concat(Or(Const?("+"), Const?("-")), rec("times")), expr, Expression.InfixBuilder()))(pos)
-    }
-
-    /* The DSL makes verification 7/2 slower (7M resource units vs 2M resource units above*/
-    /*function {:opaque} plus(functions: set<string>): (mapper: ParserMapper<Expression>)
-      requires "times" in functions
-      ensures FixMapInnerOnce("plus__", mapper, functions, |input|)
-    {
-       (rec: ParserSelector<Expression>, pos: nat)
-         requires RecSpec("plus__", functions, rec, pos) =>
-           B(rec("times")).Then((expr: Expression, pos': nat) =>
-             C?("+").o_I(B(rec("times")))
-             .Repeat(expr, Expression.BinaryBuilder("+"))).apply(pos)
-    }*/
-
-    function {:opaque} ExpressionsFix(): (r: ParseResult<Expression>)
-    {
-      var functions := {"atom", "times", "plus__"};
-      var underlying := fixmapBase[ 
-        "atom" := atom(functions)][
-        "times" := times(functions)][
-        "plus__" := plus(functions)];
-      FixMap(underlying, "plus__")(0)
-    }
-  }
-
-  function NatToString(n: nat): string {
-    if 0 <= n <= 9 then
-      ["0123456789"[n]]
-    else
-      NatToString(n/10) + NatToString(n%10)
-  }
+module ArithmeticParser {
+  import opened StringParsers
+  import opened Printer
 
   datatype Expression =
     | Binary(op: string, left: Expression, right: Expression)
@@ -85,7 +20,7 @@ module {:options "-functionSyntax:4", "-quantifierSyntax:4"}  EngineParens {
       requires level <= 2
     {
       match this
-      case Number(x) => NatToString(x)
+      case Number(x) => Printer.natToString(x)
       case Binary(op, left, right) => 
         (match level case 0 => "(" case 1 => "[" case 2 => "{")
         + left.ToString((level + 1)%3) + op + right.ToString((level + 1) % 3)
@@ -93,6 +28,9 @@ module {:options "-functionSyntax:4", "-quantifierSyntax:4"}  EngineParens {
     }
   }
 
+  const parser: Parser<Expression>
+    := Succeed<Expression>(Number(1))
+  
   function repeat(str: string, n: nat): (r: string)
     ensures |r| == |str| * n
   {
@@ -100,18 +38,23 @@ module {:options "-functionSyntax:4", "-quantifierSyntax:4"}  EngineParens {
     else str + repeat(str, n-1)
   }
 
+
   method Main(args: seq<string>) {
     if |args| <= 1 {
       return;
     }
     for i := 1 to |args| {
       var input := args[i];
-      var engine := new EngineParens(input);
-      match engine.ExpressionsFix() {
-        case PSuccess(_, n) => print "result:", n.ToString(0);
-        case PFailure(level, error, pos) => print input, "\n";
+      Succeed_NonCrashingAuto<Expression>();
+      assert Valid(parser);
+      reveal Valid();
+      match parser(input) {
+        case PSuccess(result, _) =>
+          print "result:", result.ToString(0), "\n";
+        case PFailure(level, failureData) => print input, "\n";
+          var pos: nat := |input| - |failureData.remaining|; // Need the parser to be Valid()
           print repeat(" ", pos), "^","\n";
-        print error;
+        print failureData.message;
       }
       print "\n";
     }
